\section{Logistic regression and Naive Bayes }

A common debate in machine learning has been over generative versus
discriminative models for classification.  In this question we will
explore this issue by considering Naive Bayes and logistic regression.

\begin{enumerate}
\item Naive Bayes : $P(X,Y)$ and Logistic Regression: $P(Y|X)$


\item 
\begin{align*}
	Using \; Bayes\; rule \\
	P(Y=1|X) =\dfrac{P (Y=1) * P(X | Y=1)}{P(Y=0) * P(X | Y =0) + P(Y=1)*P(X|Y=1)} \\
	Dividing \; by \; {P (Y=1) * P(X | Y=1)}\\
	= \dfrac{1}{1 + \dfrac{P(Y=0) * P(X | Y =0)} {P (Y=1) * P(X | Y=1)} } \\
	Putting \; in\; exponential \; and \; logarithms\\
	= \dfrac{1}{1 + e^{\log\left({\dfrac{P(Y=0) * P(X | Y =0)} {P (Y=1) * P(X | Y=1)} }\right)}} \\
	Since \;X \;is\; conditionally\; independent \\
	= \dfrac{1}{1 + e^{\left(\log{\left(\dfrac{P(Y=0)} {P (Y=1)}\right)} + \log {\left(\dfrac{P(X | Y=0)}{P(X | Y=1} \right)}\right)}} \\
	= \dfrac{1}{1 + e^{\left(\log{\left(\dfrac{1-\pi} {\pi}\right)} + \log {\left(\dfrac{\theta_{i0}^{X_i}*(1-\theta_{i0})^{(1-X_i)}}{\theta_{i1}^{X_i}*(1-\theta_{i1})^{(1-X_i)}} \right)}\right)}} \ldots\ldots (i)\\
	Solving \;the\; exponent \; in \; denominator \\
	= \log{\left(\theta_{i0}^{X_i} * (1-\theta_{i0})^{(1-X_i)} \right)} - \log{\left(\theta_{i1}^{X_i} * (1-\theta_{i1})^{(1-X_i)} \right)}\\
	= \log{\theta_{i0}^{X_i}} + \log{\left((1-\theta_{i0})^{(1-X_i)}\right)} - \log{\theta_{i1}^{X_i}} - \log{\left((1-\theta_{i1})^{(1-X_i)}\right)}\\
	= (1-X_i) \left[  \log{(1-\theta_{i0})} - \log{(1-\theta_{i1})} \right] + {X_i}\left[ \log{\theta_{i0}} -\log{\theta{i1}}    \right]\\
	Solving\; \\
	={X_i} \left[ \log{\theta_{i0}} - \log{\theta_{i1}} + log{(1-\theta_{i1})} - \log{(1- \theta_{i0})} \right] + \log{\left( \dfrac{(1-\theta_{i0})}{(1-\theta_{i1})} \right)} \\
	={X_i} \left[ \log{\left( \dfrac{\theta_{i0}}{\theta_{i1}} * \dfrac{1- \theta_{i1}}{1- \theta_{i0}}\right) } \right] + \log{\left( \dfrac{(1-\theta_{i0})}{(1-\theta_{i1})} \right)} \\
	Replacing \; the \; values \; in \; (i) \\
	=  \dfrac{1}{1 + e^{\left(\log{\left(\dfrac{1-\pi} {\pi}\right)} + {X_i} \left[ \log{\left( \dfrac{\theta_{i0}}{\theta_{i1}} * \dfrac{1- \theta_{i1}}{1- \theta_{i0}}\right) } \right] + \log{\left( \dfrac{(1-\theta_{i0})}{(1-\theta_{i1})} \right)}  \right)}} \\
	Rearranging \; and \; comparing \; with\; logistic \; regression \dfrac{1}{1+e^{w_0 + w_1*X_i}}\\
	w_0 + w_1*X_i =   {\left(\log{\left(\dfrac{1-\pi} {\pi}\right)} + \log{\left( \dfrac{(1-\theta_{i0})}{(1-\theta_{i1})} \right)}  \right) + {X_i} \left[ \log{\left( \dfrac{\theta_{i0}}{\theta_{i1}} * \dfrac{1- \theta_{i1}}{1- \theta_{i0}}\right) } \right] } \\
\end{align*}
\end{enumerate}
